Ed: Prove SwapConditional

code/experimental/ed25519/Hacl.Impl.Ed25519.SwapConditional.fst
@@ -24,10 +24,12 @@ val swap_conditional_step:
     (requires fun h ->
       live h a /\ live h b /\ live h out_a /\ live h out_b /\
       disjoint out_a out_b /\ disjoint a b)
-    (ensures fun h0 _ h1 -> modifies (loc out_a |+| loc out_b) h0 h1)
-//(if v swap = pow2 64 - 1 then (as_seq h1 out_a == as_seq h0 b /\ as_seq h1 out_b == as_seq h0 a)
-//else (as_seq h1 out_a == as_seq h0 a /\ as_seq h1 out_b == as_seq h0 b)) ))
+    (ensures fun h0 _ h1 -> modifies (loc out_a |+| loc out_b) h0 h1 /\
+      (if v swap = pow2 64 - 1 then (as_seq h1 out_a == as_seq h0 b /\ as_seq h1 out_b == as_seq h0 a)
+      else (as_seq h1 out_a == as_seq h0 a /\ as_seq h1 out_b == as_seq h0 b)))
+
 let swap_conditional_step a' b' a b swap =
+  let h0 = get() in
   let a0 = a.(0ul) in
   let a1 = a.(1ul) in
   let a2 = a.(2ul) in
@@ -38,11 +40,21 @@ let swap_conditional_step a' b' a b swap =
   let b2 = b.(2ul) in
   let b3 = b.(3ul) in
   let b4 = b.(4ul) in
-  let x0 = swap &. (a0 ^. b0) in
-  let x1 = swap &. (a1 ^. b1) in
-  let x2 = swap &. (a2 ^. b2) in
-  let x3 = swap &. (a3 ^. b3) in
-  let x4 = swap &. (a4 ^. b4) in
+  let x0 = (a0 ^. b0) &. swap in
+  let x1 = (a1 ^. b1) &. swap in
+  let x2 = (a2 ^. b2) &. swap in
+  let x3 = (a3 ^. b3) &. swap in
+  let x4 = (a4 ^. b4) &. swap in
+  logxor_lemma a0 b0;
+  logxor_lemma b0 a0;
+  logxor_lemma a1 b1;
+  logxor_lemma b1 a1;
+  logxor_lemma a2 b2;
+  logxor_lemma b2 a2;
+  logxor_lemma a3 b3;
+  logxor_lemma b3 a3;
+  logxor_lemma a4 b4;
+  logxor_lemma b4 a4;
   a'.(0ul) <- a0 ^. x0;
   b'.(0ul) <- b0 ^. x0;
   a'.(1ul) <- a1 ^. x1;
@@ -52,7 +64,33 @@ let swap_conditional_step a' b' a b swap =
   a'.(3ul) <- a3 ^. x3;
   b'.(3ul) <- b3 ^. x3;
   a'.(4ul) <- a4 ^. x4;
-  b'.(4ul) <- b4 ^. x4
+  b'.(4ul) <- b4 ^. x4;
+  let h1 = get() in
+  let lemma_ones () : Lemma
+    (requires v swap == pow2 64 - 1)
+    (ensures as_seq h1 a' == as_seq h0 b /\ as_seq h1 b' == as_seq h0 a)
+  = Lib.IntTypes.Compatibility.uintv_extensionality swap (ones U64 SEC);
+    logand_ones (a0 ^. b0);
+    logand_ones (a1 ^. b1);
+    logand_ones (a2 ^. b2);
+    logand_ones (a3 ^. b3);
+    logand_ones (a4 ^. b4);
+    assert (Seq.equal (as_seq h1 a') (as_seq h0 b));
+    assert (Seq.equal (as_seq h0 a) (as_seq h1 b'))
+  in
+  let lemma_zero () : Lemma
+    (requires v swap == 0)
+    (ensures as_seq h1 a' == as_seq h0 a /\ as_seq h1 b' == as_seq h0 b)
+  = logand_zeros (a0 ^. b0);
+    logand_zeros (a1 ^. b1);
+    logand_zeros (a2 ^. b2);
+    logand_zeros (a3 ^. b3);
+    logand_zeros (a4 ^. b4);
+    assert (Seq.equal (as_seq h1 a') (as_seq h0 a));
+    assert (Seq.equal (as_seq h0 b) (as_seq h1 b'))
+  in
+  Classical.move_requires lemma_zero ();
+  Classical.move_requires lemma_ones ()
 
 val swap_conditional:
     out_a:point
@@ -73,15 +111,15 @@ val swap_conditional:
       Spec.Ed25519.cswap2 (to_u8 i) (F51.point_eval h0 a) (F51.point_eval h0 b)
     )
 
-//      (if v i = 1 then (as_seq h1 out_a == as_seq h0 b /\ as_seq h1 out_b == as_seq h0 a)
-//         else (as_seq h1 out_a == as_seq h0 a /\ as_seq h1 out_b == as_seq h0 b))
+#set-options "--z3rlimit 50"
+
 let swap_conditional a' b' a b iswap =
   let swap = u64 0 -. iswap in
+  Math.Lemmas.small_mod (v iswap) (pow2 8);
   swap_conditional_step (getx a') (getx b') (getx a) (getx b) swap;
   swap_conditional_step (gety a') (gety b') (gety a) (gety b) swap;
   swap_conditional_step (getz a') (getz b') (getz a) (getz b) swap;
-  swap_conditional_step (gett a') (gett b') (gett a) (gett b) swap;
-  admit()
+  swap_conditional_step (gett a') (gett b') (gett a) (gett b) swap
 
 val swap_conditional_inplace:
     a:point
@@ -98,8 +136,8 @@ val swap_conditional_inplace:
     )
 let swap_conditional_inplace a b iswap =
   let swap = u64 0 -. iswap in
+  Math.Lemmas.small_mod (v iswap) (pow2 8);
   swap_conditional_step (getx a) (getx b) (getx a) (getx b) swap;
   swap_conditional_step (gety a) (gety b) (gety a) (gety b) swap;
   swap_conditional_step (getz a) (getz b) (getz a) (getz b) swap;
-  swap_conditional_step (gett a) (gett b) (gett a) (gett b) swap;
-  admit()
+  swap_conditional_step (gett a) (gett b) (gett a) (gett b) swap
